 %%%%%%%%%%%%%%%%%%%%%%%%%%%%%%%%%%%%%%%%%%%%%%%%%
%%%%%%%%%%%%%%%%%%%%%%%%%%%%%%%%%%%%%%%%%%%%%%%%%
%%%      IGNORE THIS FIRST PART        %%%%%%%%%%   EXCEPT TO ENTER/DELETE YOUR NAME WHERE INDICATED
%%%%%%%%%%%%%%%%%%%%%%%%%%%%%%%%%%%%%%%%%%%%%%%%%
%%%%%%%%%%%%%%%%%%%%%%%%%%%%%%%%%%%%%%%%%%%%%%%%%

\documentclass[12pt]{amsart}
\usepackage{amsmath, amssymb, amsthm}
\usepackage{mathrsfs}
\usepackage{array}
\usepackage{enumitem}
\usepackage[usenames,dvipsnames]{xcolor}
\usepackage{graphicx}
\usepackage{fancyhdr}
\usepackage{caption}
\usepackage{hyperref}
\usepackage[labelformat=simple]{subcaption}
\usepackage[framemethod=default]{mdframed}
\usepackage{framed}
\usepackage{setspace}
\usepackage{changepage}

\setlength{\parindent}{0pt}

\newmdenv[linecolor=NavyBlue,backgroundcolor=White]{myframe}
\renewcommand\thesubfigure{(\Alph{subfigure})}
\renewcommand\thesubfigure{(\Alph{subfigure})}

\newcounter{problem_number}[section]
\newcommand{\num}{\refstepcounter{problem_number}\arabic{problem_number}}
\newcommand{\numlabel}[1]{\refstepcounter{problem_number}\label{#1}\arabic{problem_number}}

\newtheorem*{theorem}{Theorem}
\newtheoremstyle{named}{}{}{\itshape}{}{\bfseries}{.}{.5em}{\thmnote{#3}}
\theoremstyle{named}
\newtheorem*{namedtheorem}{Theorem}

\newenvironment{prf}
{\medskip\begin{color}{Gray}\begin{framed}\begin{color}{NavyBlue}\begin{proof}[Proof]
\doublespacing}
{\end{proof}\end{color}\end{framed}\end{color}\medskip}

\newenvironment{soln}
{\begin{color}{Gray}\begin{framed}\begin{color}{NavyBlue}\begin{proof}[Solution]
\doublespacing}
{\end{proof}\end{color}\end{framed}\end{color}}

\theoremstyle{definition}
\newtheorem{problem}{Problem}
\newtheorem{proposition}{Proposition}

\setenumerate[1]{label=(\roman*)}

\newcommand{\jeff}[1]{\textbf{\textcolor{WildStrawberry}{#1}}}
\newcommand{\student}[1]{\textbf{\textcolor{Orange}{#1}}}
\newcommand{\peer}[1]{\textbf{\textcolor{ForestGreen}{#1}}}

\textwidth=6.5in
\hoffset-.75in
\textheight=9in
\voffset-.75in
\footskip=30pt
\headheight=14pt
\pagestyle{fancy}
\lhead{\emph{\textcolor{Gray}{Homework \#7}}}			%%  UPDATE THE VERSION HERE!!!
\rhead{\emph{\textcolor{Gray}{Seven Lewis}}}			%%  ENTER/DELETE YOUR NAME HERE!!!
\chead{\emph{\textcolor{Gray}{MATH 309}}}
\cfoot{\thepage}
\renewcommand{\headrulewidth}{0.35pt}
\renewcommand{\footrulewidth}{0.35pt}
\thispagestyle{fancy}

%%%%%%%%%%%%%%%%%%%%%%%%%%%%%%%%%%%%%%%%%%%%%%%%%
%%%%%%%%%%%%%%%%%%%%%%%%%%%%%%%%%%%%%%%%%%%%%%%%%
%%%       ADD CUSTOM COMMANDS HERE     %%%%%%%%%%
%%%%%%%%%%%%%%%%%%%%%%%%%%%%%%%%%%%%%%%%%%%%%%%%%
%%%%%%%%%%%%%%%%%%%%%%%%%%%%%%%%%%%%%%%%%%%%%%%%%

\newcommand{\F}{\mathbb F}
\newcommand{\N}{\mathbb N}
\newcommand{\Q}{\mathbb Q}
\newcommand{\R}{\mathbb R}
\renewcommand{\S}{\mathbb S}
\newcommand{\Z}{\mathbb Z}
\newcommand{\RP}{\mathbb{RP}}

\newcommand{\Ll}{\mathcal L}
\newcommand{\Pp}{\mathcal P}
\newcommand{\Rr}{\mathcal R}

\newcommand{\Line}[1]{\overleftrightarrow{#1}}
\newcommand{\Ray}[1]{\overrightarrow{#1}}

%%%%%%%%%%%%%%%%%%%%%%%%%%%%%%%%%%%%%%%%%%%%%%%%%
%%%%%%%%%%%%%%%%%%%%%%%%%%%%%%%%%%%%%%%%%%%%%%%%%
%%%       NOW THE DOCUMENT BEGINS      %%%%%%%%%%
%%%%%%%%%%%%%%%%%%%%%%%%%%%%%%%%%%%%%%%%%%%%%%%%%
%%%%%%%%%%%%%%%%%%%%%%%%%%%%%%%%%%%%%%%%%%%%%%%%%

\begin{document}

Prove the following propositions. Format your proof so each step of the proof is on its own line; each line should still be a complete sentence. Below, I have entered a nonsensical proof as a model.

%%%%%%%%%%%%%%%%%%%%%%%%%%%%%%%%%%%%%%%%%%%%%%%%%%%%%%%%%%%%%%%%%%%%%%%%%%%%%%
\begin{proposition}
	Suppose $a,b,c\in\Z$.
	If $a^2+b^2=c^2$, then $a$ or $b$ is even.
\end{proposition}

\begin{prf}
	\phantom{ }

	% Lemma: All integers $a$ have the same parity as $a^2$.

	% \begin{adjustwidth}{2em}{0em} 
	% 	\textbf{Case 1:} $a$ is even.
		
	% 	\begin{adjustwidth}{2em}{0em} 
	% 		Then $a = 2x$ for some integer $x$.

	% 		Expression $a^2$ becomes $(2x)^2 = 4x^2 = 2(2x^2)$.
			
	% 		So $a^2 = 2y$ where $y$ is the integer $2x^2$.

	% 		Thus, $a^2$ is even.
	% 	\end{adjustwidth}

	% 	\textbf{Case 2:} $a$ is odd.

	% 	\begin{adjustwidth}{2em}{0em} 
	% 		Then $a = 2x + 1$ for some integer $x$.

	% 		Expression $a^2$ becomes $(2x+1)^2 = 4x^2+4x+1 = 2(2x^2+2x)+1$.

	% 		So $a^2 = 2y + 1$ where $y$ is the integer $2x^2+2x$.
			
	% 		Thus, $a^2$ is odd. 
	% 	\end{adjustwidth}
		
	% \end{adjustwidth}
	Let $a,b,c \in \mathbb Z$. 
	
	Suppose $a^2 + b^2 = c^2$ and it's 
	not the case that $a$ or $b$ is even.

	Therefore, $a$ and $b$ are both odd.

	So $a = 2x + 1$ and $b = 2y + 1$ for some integers $x$ and $y$.

	Either $c$ is even or odd.

	\textbf{Case 1:} $c$ is even.
	\begin{adjustwidth}{2em}{0em} 
		Then $c = 2z$ for some integer $z$.

		The expression $a^2 + b^2 = c^2$ becomes $(2x + 1)^2 + (2y+1)^2 = 4z^2$.

		Expanding the expression yields $4x^2 + 4x + 1 + 4y^2 + 4y + 1 = 4z^2$.

		Factoring yields $4(x^2+y^2+x+y)+2 = 4z^2$.

		Simplifying the expression shows $4k + 2 = 4j$ where $k$ and $j$ are
		the integers $x^2+y^2+x+y$ and $4z^2$ respectfully. 

		Observe that $2 = 4(k - j) \implies 2 = 4l$ where $l$ is the integer $k-j$, thus $4|2$.
		
		We have arrived at contradiction.
	\end{adjustwidth}

	\textbf{Case 2:} $c$ is odd.
	\begin{adjustwidth}{2em}{0em}
		Then $c = 2z + 1$ for some integer $x$.

		The expression $a^2 + b^2 = c^2$ becomes $(2x + 1)^2 + (2y+1)^2 = (2z+1)^2$.

		Expanded and factored yields $2(2x^2 + 2x + 2y^2 + 2y + 1) = 2(2z^2 + 2z) + 1$

		Simplifying the expression shows that $2k = 2j + 1$ for integers $k$ and $j$.

		Therefore, an even number equals an odd number. 
		
		We have arrived at contradiction.
	\end{adjustwidth}
\end{prf}

\phantom{ }

\phantom{ }

\phantom{ }

\phantom{ }
%%%%%%%%%%%%%%%%%%%%%%%%%%%%%%%%%%%%%%%%%%%%%%%%%%%%%%%%%%%%%%%%%%%%%%%%%%%%%%
\begin{proposition}
	Suppose $x,y\in\Z$.
	If $x+y$ is even, then $x$ and $y$ have the same parity.
\end{proposition}

\begin{prf}
	\phantom{ }

	Let $x,y \in \mathbb Z$.
	
	Suppose $x$ and $y$ do not have the same parity.

	% Observe that $x$ and $y$ either have the same parity or they do not.

	Then $x$ is even and $y$ odd without loss of generality.

	So $x = 2a$ and $y = 2b + 1$ for some integers $a$ and $b$.

	The expression $x + y$ becomes $2a + 2b + 1 = 2(a+b) + 1$.

	Therefore $x + y = 2m + 1$ where $m$ is the integer $a+b$.

	So, $x + y$ is odd.
\end{prf}

%%%%%%%%%%%%%%%%%%%%%%%%%%%%%%%%%%%%%%%%%%%%%%%%%%%%%%%%%%%%%%%%%%%%%%%%%%%%%%
\begin{proposition}
	If $a\equiv b\pmod n$, then $\gcd(a,n) = \gcd(b,n)$.
\end{proposition}

\begin{prf}
	\phantom{ }

	Let $a,b \in \mathbb Z$ and $n \in \mathbb N$. 

	Suppose $a \equiv b (\text{mod } n)$.

	Then $n|(a-b)$.

	Then $nx = a-b$ for some integer $x$.

	The division algorithm states that:

	\begin{adjustwidth}{2em}{0em}
		$a = nq_1 + r_1$ where $q_1, r_1 \in \mathbb Z$ where $0 \leq r_1 < n$.

		$b = nq_2 + r_2$ where $q_2, r_2 \in \mathbb Z$ where $0 \leq r_2 < n$.
	\end{adjustwidth}

	So, $nx = nq_1 + r_1 - nq_2 - r_2$

	\hspace{3.15em}$= n(q_1 - q_2) + r_1 - r_2$

	Observe that $r_1 - r_2$ must be some multiple of $n$ in order for the equality to hold.

	So, $ny = r_1-r_2$.

	However, $-n < r_1 - r_2 < n$, so the only possible multiple is $0$.

	So, $n(0) = 0 = r_1-r_2 \implies r_1 = r_2$.

	Therefore they share the same remainder. Moving forward: Let $r = r_1 = r_2$.

	If $r = 0$, then both $a$ and $b$ are multiples of $n$. So the greatest shared divisor
	between $a$ and $n$ and between $b$ and $n$ will simply be $n$ itself. 

	So, $\text{gcd}(a,n) = \text{gcd}(b,n)$ when $r = 0$. 

	If $r \neq 0$, then $n$ and $r$ may share prime factors, we can factor these out and 
	replace them with their product $p$:
	\begin{adjustwidth}{2em}{0em}
		$a = p(n'q_1+r')$

		$b = p(n'q_2+r')$
	\end{adjustwidth}

	Where $n = pn'$ and $r = pr'$.

	\textbf{Lemma:} Let $\alpha, \beta \in \mathbb N$, $x \in \mathbb Z$. If $\alpha$ and $\beta$ are 
	coprime, then $\text{gcd}(\alpha x+\beta,\alpha) = 1$.

	\begin{adjustwidth}{2em}{0em}		
		Suppose $\text{gcd}(\alpha x+\beta ,\alpha) \neq 1$.

		Then $\text{gcd}(\alpha +\beta ,\alpha) > 1$.

		So, $\alpha x+\beta $ and $\alpha$ share some common divisor $d$.

		It follows that $d|\alpha x+\beta $ and $d|\alpha$.

		Expanded, this is $dm_1 = \alpha x +\beta $ and $dm_2 = \alpha$.

		Substituting $\alpha$, $dm_1 = \alpha x+\beta  \implies dm_1 = dm_2x+\beta $.

		Isolation $\beta $, we get $\beta  = dm_1 - dm_2x \implies \beta  = d(m_1-m_2x)$.

		Thus, $dm_3 = \beta $ where $m_3$ is the integer $m_1-m_2x$.

		So, $d|\beta $. 

		Because $d|\beta $ and $d|\alpha$ for some $d > 0$, $\beta$ and $\alpha$ cannot
		be coprime.
	\end{adjustwidth}

	So, $\text{gcd}(n'q+r',n') = 1$ when $q \in \{q_1,q_2\}$, because $n'$ and $r'$ are coprime. 

	So, $n'q+r'$ and $n'$ share no prime factors.

	Since $a = p(n'q_1+r')$, 
	$n = pn'$, and $n'q_1+r'$ and $n'$ share no more common factors, it follows that 
	$\text{gcd}(a,n) = p$.

	Similarly, since $b = p(n'q_2+r')$, $n = pn'$, and $n'q_2+r'$ and $n'$ 
	share no more common factors, it follows that $\text{gcd}(b,n) = p$.

	So, $\text{gcd}(a,n) = \text{gcd}(b,n)$ when $r \neq 0$. 
	% $\text{gcd}(a,n) = \text{ }$greatest $x$ where $x|a$ and $x|n$. 

	% $\text{gcd}(b,n) = \text{ }$greatest $x$ where $x|b$ and $x|n$.
	
	% So, there exists some $x$ and $y$ where $x \neq y$, $x|a$, $x|n$, $y|b$, $y|n$.
\end{prf}
%%%%%%%%%%%%%%%%%%%%%%%%%%%%%%%%%%%%%%%%%%%%%%%%%%%%%%%%%%%%%%%%%%%%%%%%%%%%%%

\end{document}